Lean4Lean/Verify/Typing/ConditionallyTyped.lean
@@ -7,6 +7,10 @@ def ConditionallyTyped
     (ngen : NameGenerator) (env : VEnv) (Us : List Name) (Δ : VLCtx) (e : Expr) : Prop :=
   Closed e ∧ FVarsIn ngen.Reserves e ∧ (FVarsIn (· ∈ Δ.fvars) e → ∃ e', TrExprS env Us Δ e e')
 
+theorem ConditionallyTyped.mk {Δ : VLCtx}
+    (noBV : Δ.NoBV) (r : FVarsIn ngen.Reserves e) (H : TrExprS env Us Δ e e') :
+    ConditionallyTyped ngen env Us Δ e := ⟨noBV ▸ H.closed, r, fun _ => ⟨_, H⟩⟩
+
 theorem ConditionallyTyped.mono (H : ngen₁ ≤ ngen₂) :
     ConditionallyTyped ngen₁ env Us Δ e → ConditionallyTyped ngen₂ env Us Δ e
   | ⟨h1, h2, h3⟩ => ⟨h1, h2.mono fun _ h => h.mono H, h3⟩
@@ -21,23 +25,25 @@ theorem ConditionallyTyped.weakN_inv
   exact TrExprS.weakFV_inv henv (.skip_fvar _ _ .refl) (.refl henv hΔ) h H.1 H2
 
 theorem ConditionallyTyped.fresh
-    (henv : Ordered env) (hΔ : VLCtx.WF env Us.length ((some ⟨ngen.curr⟩, d) :: Δ))
+    (henv : Ordered env) (hΔ : VLCtx.WF env Us.length ((some (⟨ngen.curr⟩, deps), d) :: Δ))
     (H : ConditionallyTyped ngen env Us Δ e) :
-    ConditionallyTyped ngen env Us ((some ⟨ngen.curr⟩, d) :: Δ) e := by
+    ConditionallyTyped ngen env Us ((some (⟨ngen.curr⟩, deps), d) :: Δ) e := by
   refine have ⟨H1, H2, H3⟩ := H; ⟨H1, H2, fun H4 => ?_⟩
   refine have ⟨_, h⟩ := H3 (H4.mp ?_ H2); ⟨_, h.weakFV henv (.skip_fvar _ _ .refl) hΔ⟩
   intro _ h1 h2; simp at h1; rcases h1 with rfl | h1
   · cases Nat.lt_irrefl _ (h2 _ rfl)
   · exact h1
 
-def TrHasType (env : VEnv) (Us : List Name) (Δ : VLCtx) (e A : Expr) : Prop :=
-  (∀ P, IsFVarUpSet P Δ → FVarsIn P e → FVarsIn P A) ∧
-  ∃ e' A', TrExprS env Us Δ e e' ∧ TrExprS env Us Δ A A' ∧ env.HasType Us.length Δ.toCtx e' A'
-
 def ConditionallyHasType
     (ngen : NameGenerator) (env : VEnv) (Us : List Name) (Δ : VLCtx) (e A : Expr) : Prop :=
   Closed e ∧ FVarsIn ngen.Reserves e ∧ Closed A ∧ FVarsIn ngen.Reserves A ∧
-    (FVarsIn (· ∈ Δ.fvars) e → TrHasType env Us Δ e A)
+    (FVarsIn (· ∈ Δ.fvars) e → ∃ e' A', TrTyping env Us Δ e A e' A')
+
+theorem ConditionallyHasType.mk {Δ : VLCtx}
+    (noBV : Δ.NoBV) (he : TrTyping env Us Δ e A e' A')
+    (re : FVarsIn ngen.Reserves e) (rA : FVarsIn ngen.Reserves A) :
+    ConditionallyHasType ngen env Us Δ e A := by
+  refine ⟨noBV ▸ he.2.1.closed, re, noBV ▸ he.2.2.1.closed, rA, fun _ => ⟨_, _, he.1, he.2⟩⟩
 
 theorem ConditionallyHasType.typed :
     ConditionallyHasType ngen env Us Δ e A → ConditionallyTyped ngen env Us Δ e
@@ -53,29 +59,33 @@ theorem ConditionallyHasType.weakN_inv
     ConditionallyHasType ngen env Us Δ e A := by
   have ⟨c1, f1, c2, f2, H⟩ := H
   refine ⟨c1, f1, c2, f2, fun H4 => ?_⟩
-  have ⟨h1, e', A', h2, h3, h4⟩ := H H4.fvars_cons
+  have ⟨e', A', h1, h2, h3, h4⟩ := H H4.fvars_cons
   have W : VLCtx.FVLift Δ ((some fv, d) :: Δ) 0 (0 + d.depth) 0 := .skip_fvar _ _ .refl
   have ⟨e'', he⟩ := TrExprS.weakFV_inv henv W (.refl henv hΔ) h2 c1 H4
   have ee := h2.uniq henv (.refl henv hΔ) <| he.weakFV henv W hΔ
-  have : IsFVarUpSet (· ∈ VLCtx.fvars Δ) ((some fv, d) :: Δ) := ⟨(hΔ.2.1 _ rfl).elim, .fvars⟩
+  have := hΔ.2.1 _ _ rfl
+  have : IsFVarUpSet (· ∈ VLCtx.fvars Δ) ((some fv, d) :: Δ) :=
+    ⟨(hΔ.2.1 _ _ rfl).1.elim, .fvars hΔ.1.fvwf⟩
   have ⟨_, hA⟩ := TrExprS.weakFV_inv henv W (.refl henv hΔ) h3 c2 <| h1 _ this H4
   have AA := h3.uniq henv (.refl henv hΔ) <| hA.weakFV henv W hΔ
   have h4 := h4.defeqU_r henv hΔ.toCtx AA |>.defeqU_l henv hΔ.toCtx ee
   have h4 := (HasType.weakN_iff henv hΔ.toCtx W.toCtx).1 h4
-  refine ⟨fun P hP he' => ?_, _, _, he, hA, h4⟩
+  refine ⟨_, _, fun P hP he' => ?_, he, hA, h4⟩
   exact h1 _
-    ⟨fun h => (hΔ.2.1 _ rfl).elim h.2, IsFVarUpSet.and_fvars.1 hP⟩
+    ⟨fun h => (hΔ.2.1 _ _ rfl).1.elim h.2, (IsFVarUpSet.and_fvars hΔ.1.fvwf).1 hP⟩
     (he'.mp (fun _ => .intro) he.fvarsIn) |>.mono fun _ => (·.1)
 
 theorem ConditionallyHasType.fresh
-    (henv : Ordered env) (hΔ : VLCtx.WF env Us.length ((some ⟨ngen.curr⟩, d) :: Δ))
+    (henv : Ordered env)
+    (hΔ : VLCtx.WF env Us.length ((some (⟨ngen.curr⟩, deps), d) :: Δ))
     (H : ConditionallyHasType ngen env Us Δ e A) :
-    ConditionallyHasType ngen env Us ((some ⟨ngen.curr⟩, d) :: Δ) e A := by
+    ConditionallyHasType ngen env Us ((some (⟨ngen.curr⟩, deps), d) :: Δ) e A := by
   refine have ⟨c1, f1, c2, f2, H⟩ := H; ⟨c1, f1, c2, f2, fun H4 => ?_⟩
-  have ⟨h1, _, _, h2, h3, h4⟩ := H (H4.mp ?_ f1)
-  · have W : VLCtx.FVLift Δ ((some ⟨ngen.curr⟩, d) :: Δ) 0 (0 + d.depth) 0 := .skip_fvar _ _ .refl
-    refine ⟨fun P hP => h1 _ hP.2, ?_⟩
-    exact ⟨_, _, h2.weakFV henv W hΔ, h3.weakFV henv W hΔ, h4.weakN henv W.toCtx⟩
+  have ⟨_, _, h1, h2, h3, h4⟩ := H (H4.mp ?_ f1)
+  · have W : VLCtx.FVLift Δ ((some (⟨ngen.curr⟩, deps), d) :: Δ) 0 (0 + d.depth) 0 :=
+      .skip_fvar _ _ .refl
+    exact ⟨_, _, fun P hP => h1 _ hP.2,
+      h2.weakFV henv W hΔ, h3.weakFV henv W hΔ, h4.weakN henv W.toCtx⟩
   · intro _ h1 h2; simp at h1; rcases h1 with rfl | h1
     · cases Nat.lt_irrefl _ (h2 _ rfl)
     · exact h1
